introduce LargerBallotsPromiseQrms invariant

paxos/proof.dfy
@@ -222,13 +222,27 @@ predicate Agreement_Inv_Lemma(c:Constants, ds:DistrSys)
 {
     && c.WF()
     && ds.WF(c)
+    && LeaderPromisesSet(c, ds)
     && (forall v, b, i | c.ValidLdrIdx(i) && LeaderIdxDecidedV(c, ds, i, v, b)
         ::  && LargerBallotsDecideV(c, ds, v, b)
+            
+            && LargerBallotsPromiseQrms(c, ds, v, b)
             && LargerBallotPhase2LeadersV(c, ds, v, b)
             // && (exists q :: QuorumOfAcceptors(c, q) && QuorumOfAcceptorsAcceptedBV(c, ds, q, v, b))
             && LargerBallotAcceptors(c, ds, v, b)
             && LargerBallotPromiseMsgs(c, ds, v, b)
             && LargerBallotProposalMsgs(c, ds, v, b)
+    )
+}
+
+
+predicate LeaderPromisesSet(c:Constants, ds:DistrSys) 
+    requires c.WF() && ds.WF(c)
+{
+    forall i | c.ValidLdrIdx(i) :: (
+        forall p | p in ds.leaders[i].promises :: 
+            && p in ds.network.sentPackets
+            && p.msg.Promise?
     )
 }
 
@@ -242,6 +256,18 @@ predicate LargerBallotsDecideV(c:Constants, ds:DistrSys, v:Value, b:Ballot)
         && c.ValidLdrIdx(i') && BalLtEq(b, b') 
         && LeaderHasDecided(c, i', ds) && LeaderHasBallotB(c, i', ds, b') 
     :: LeaderHasValueV(c, i', ds, v)
+}
+
+
+/* If v is decided with ballot b, then all Promise quorums for ballots
+* b' >= b must come from an acceptor that accepted (v, b) */
+predicate LargerBallotsPromiseQrms(c:Constants, ds:DistrSys, v:Value, b:Ballot) 
+    requires c.WF() && ds.WF(c)
+{
+    forall b' | BalLtEq(b, b') 
+    :: (forall qrm:set<Packet> | QuorumOfPromiseMsgs(c, ds, qrm, b') 
+        :: exists p :: p in qrm && BalLtEq(b, p.msg.vb.b) 
+    )
 }
 
 /* If v is decided with ballot b, then all phase 2 leaders with ballots
@@ -300,18 +326,22 @@ lemma NextPreservesAgreementInvLemma(c:Constants, ds:DistrSys, ds':DistrSys)
     requires Next(c, ds, ds')
     ensures Agreement_Inv_Lemma(c, ds')
 {
+    assert LeaderPromisesSet(c, ds');
     if exists v, b, i :: c.ValidLdrIdx(i) && LeaderIdxDecidedV(c, ds, i, v, b) {
         var v, b, i :| c.ValidLdrIdx(i) && LeaderIdxDecidedV(c, ds, i, v, b);
-        
         Lemma_LargerBallotAcceptors_1(c, ds, ds', i, v, b);
-        assert LargerBallotAcceptors(c, ds', v, b);
-
+        assert LargerBallotAcceptors(c, ds', v, b);     // Done
         Lemma_LargerBallotsDecideV_1(c, ds, ds', i, v, b);
-        assert LargerBallotsDecideV(c, ds', v, b);
+        assert LargerBallotsDecideV(c, ds', v, b);      // Done
+        assume LargerBallotsPromiseQrms(c, ds', v, b);  // TODO: Assume this for now
+        
 
-        assume false;
+        Lemma_LargerBallotPhase2LeadersV_1(c, ds, ds', i, v, b);
         assert LargerBallotPhase2LeadersV(c, ds', v, b);
-        // assert (exists q :: QuorumOfAcceptors(c, q) && QuorumOfAcceptorsAcceptedBV(c, ds, q, v, b))
+
+        // TODO
+        assume false;
+        // assert (exists q :: QuorumOfAcceptors(c, q) && QuorumOfAcceptorsAcceptedBV(c, ds, q, v, b));
         assert LargerBallotAcceptors(c, ds', v, b);
         assert LargerBallotPromiseMsgs(c, ds', v, b);
         assert LargerBallotProposalMsgs(c, ds', v, b);
@@ -336,6 +366,17 @@ lemma Lemma_LargerBallotsDecideV_1(c:Constants, ds:DistrSys, ds':DistrSys,i:int,
     requires c.ValidLdrIdx(i) && LeaderIdxDecidedV(c, ds, i, v, b)
     ensures LargerBallotsDecideV(c, ds', v, b)
 {}
+
+lemma Lemma_LargerBallotPhase2LeadersV_1(c:Constants, ds:DistrSys, ds':DistrSys,i:int, v:Value, b:Ballot) 
+    requires Agreement_Inv_Lemma(c, ds)
+    requires Next(c, ds, ds')
+    requires c.ValidLdrIdx(i) && LeaderIdxDecidedV(c, ds, i, v, b)
+    ensures LargerBallotPhase2LeadersV(c, ds', v, b)
+{
+    // TODO
+
+}
+
 
 
 
